Utils/sets.v
@@ -440,10 +440,6 @@ induction n.
     assumption.
 Qed.
 
-Section Set_of_tuple_of_positive.
-
-Context {Ar : Arity}.
-
 Fixpoint eqList (l1 l2 : list positive) :=
   match l1, l2 with
     | nil         , nil          => True
@@ -624,6 +620,16 @@ rewrite H; auto; clear H; elim (IHl1 l2); intro H;
 [apply CompEq; split|apply CompLt|apply CompGt]; auto; apply Pos.eq_refl.
 Qed.
 
+Lemma eqListOK : forall l1 l2, eqList l1 l2 -> l1 = l2.
+Proof.
+intro l1; induction l1; intro l2; induction l2; simpl; try solve [intuition].
+intros [Hhd Htl]; rewrite Hhd, (IHl1 l2); [reflexivity|auto].
+Qed.
+
+Section Set_of_tuple_of_positive.
+
+Context {Ar : Arity}.
+
 Definition tST := cartesianPower positive (Datatypes.S (Datatypes.S n)).
 
 Definition eqST (cp1 cp2 : tST) :=
@@ -686,20 +692,12 @@ exact (Build_OrderedType eqST eqbST ltST compareST
                          CompareST).
 Defined.
 
-(*
 Lemma eqListSortOCP : forall (cp : tST),
   eqList (CPToList (OCP cp)) (sort (CPToList cp)).
 Proof.
 intro cp; unfold OCP, OCPAux; elim_eq_rect; simpl.
 rewrite CPLOK; apply eqListRefl.
 Qed.
-
-Lemma eqListOK : forall l1 l2, eqList l1 l2 -> l1 = l2.
-Proof.
-intro l1; induction l1; intro l2; induction l2; simpl; try solve [intuition].
-intros [Hhd Htl]; rewrite Hhd, (IHl1 l2); [reflexivity|auto].
-Qed.
-*)
 
 (*
 TODO: try to see if using sorted lists would not make the tactic faster.
